
format-version: 1.2
import: http://purl.obolibrary.org/obo/lsfo/imports/cob_import.owl
ontology: lsfo
property_value: http://purl.org/dc/terms/description "None" xsd:string
property_value: http://purl.org/dc/terms/title "Light Source Facility Ontology" xsd:string
property_value: http://purl.org/dc/terms/license https://creativecommons.org/licenses/unspecified


[Term]
id: LSFO:0000000
name: root node

[Term]
id: LSFO:7770001
name: Experiment
def: "A specific experimental run or investigation conducted at a light source facility." [https://pmc.ncbi.nlm.nih.gov/articles/PMC12000454/]
is_a: LSFO:0000000 ! root node

[Term]
id: LSFO:7770002
name: Beamline
def: "An experimental station and its beam delivery system at a light source facility." [https://pmc.ncbi.nlm.nih.gov/articles/PMC12000454/]
is_a: LSFO:0000000 ! root node

[Term]
id: LSFO:7770003
name: Beam
def: "The radiation beam used in an experiment, with properties like energy and polarization." [https://als.lbl.gov/beamlines/4-0-2/]
is_a: LSFO:0000000 ! root node

[Term]
id: LSFO:7770004
name: Sample
def: "The material sample or specimen studied in an experiment." [https://pmc.ncbi.nlm.nih.gov/articles/PMC12000454/]
is_a: LSFO:0000000 ! root node

[Term]
id: LSFO:7770005
name: Experimental apparatus
def: "The equipment used in an experiment, including detectors and sample environments." [https://pmc.ncbi.nlm.nih.gov/articles/PMC12000454/]
is_a: LSFO:0000000 ! root node

[Term]
id: LSFO:7770006
name: Detector
def: "An instrument capturing data in an experiment, such as a camera or spectrometer." [https://pmc.ncbi.nlm.nih.gov/articles/PMC12000454/]
is_a: LSFO:7770005 ! Experimental apparatus

[Term]
id: LSFO:7770007
name: Sample environment
def: "Apparatus controlling conditions during an experiment, such as a cryostat or pressure cell." [https://pmc.ncbi.nlm.nih.gov/articles/PMC12000454/]
is_a: LSFO:7770005 ! Experimental apparatus

[Term]
id: LSFO:7770008
name: Experimental condition
def: "Ambient or controlled conditions during an experimental run, such as temperature or pressure." [https://pmc.ncbi.nlm.nih.gov/articles/PMC12000454/]
is_a: LSFO:0000000 ! root node

[Term]
id: LSFO:7770009
name: Experiment metadata
def: "Additional contextual information about an experiment, such as purpose, operator, date, or scheduling information." [https://pmc.ncbi.nlm.nih.gov/articles/PMC12000454/]
is_a: LSFO:0000000 ! root node

[Term]
id: LSFO:7770010
name: Raw data
def: "The primary data collected in an experiment, such as images, spectra, or diffraction patterns." [https://pmc.ncbi.nlm.nih.gov/articles/PMC12000454/]
is_a: LSFO:0000000 ! root node

[Term]
id: LSFO:7770011
name: Processed data
def: "Data that has been processed or analyzed from raw data." [https://pmc.ncbi.nlm.nih.gov/articles/PMC12000454/]
is_a: LSFO:0000000 ! root node

[Term]
id: LSFO:7770012
name: Analysis method
def: "The data analysis or processing method applied to raw data, which produces processed data." [https://pmc.ncbi.nlm.nih.gov/articles/PMC12000454/]
is_a: LSFO:0000000 ! root node

[Typedef]
id: LSFO:7770101
name: has_beamline
def: "Relation between an experiment and the beamline where it was conducted." [https://pmc.ncbi.nlm.nih.gov/articles/PMC12000454/]
domain: LSFO:7770001 ! Experiment
range: LSFO:7770002 ! Beamline

[Typedef]
id: LSFO:7770102
name: has_beam
def: "Relation between an experiment and the radiation beam used." [https://pmc.ncbi.nlm.nih.gov/articles/PMC12000454/]
domain: LSFO:7770001 ! Experiment
range: LSFO:7770003 ! Beam

[Typedef]
id: LSFO:7770103
name: has_sample
def: "Relation between an experiment and the material sample studied." [https://pmc.ncbi.nlm.nih.gov/articles/PMC12000454/]
domain: LSFO:7770001 ! Experiment
range: LSFO:7770004 ! Sample

[Typedef]
id: LSFO:7770104
name: has_apparatus
def: "Relation between an experiment and the experimental apparatus used." [https://pmc.ncbi.nlm.nih.gov/articles/PMC12000454/]
domain: LSFO:7770001 ! Experiment
range: LSFO:7770005 ! Experimental apparatus

[Typedef]
id: LSFO:7770105
name: has_condition
def: "Relation between an experiment and the experimental conditions." [https://pmc.ncbi.nlm.nih.gov/articles/PMC12000454/]
domain: LSFO:7770001 ! Experiment
range: LSFO:7770008 ! Experimental condition

[Typedef]
id: LSFO:7770106
name: has_metadata
def: "Relation between an experiment and its metadata." [https://pmc.ncbi.nlm.nih.gov/articles/PMC12000454/]
domain: LSFO:7770001 ! Experiment
range: LSFO:7770009 ! Experiment metadata

[Typedef]
id: LSFO:7770107
name: has_output
def: "Relation between an experiment and the raw data it produces." [https://pmc.ncbi.nlm.nih.gov/articles/PMC12000454/]
domain: LSFO:7770001 ! Experiment
range: LSFO:7770010 ! Raw data

[Typedef]
id: LSFO:7770108
name: derived_into
def: "Relation between raw data and the processed data derived from it." [https://pmc.ncbi.nlm.nih.gov/articles/PMC12000454/]
domain: LSFO:7770010 ! Raw data
range: LSFO:7770011 ! Processed data

[Typedef]
id: LSFO:7770109
name: has_analysis
def: "Relation between an experiment and the analysis method applied." [https://pmc.ncbi.nlm.nih.gov/articles/PMC12000454/]
domain: LSFO:7770001 ! Experiment
range: LSFO:7770012 ! Analysis method

[Typedef]
id: http://purl.org/dc/terms/description
name: description
is_metadata_tag: true

[Typedef]
id: http://purl.org/dc/terms/license
name: license
is_metadata_tag: true

[Typedef]
id: http://purl.org/dc/terms/title
name: title
is_metadata_tag: true

